modifies proofs to incorporate compositional CSD model
possible experimental approach that might make it easier to generate varied CSDs using qwen that are yet still simple enough to check the validity of.

files modified/added:
1. VerifiedAgentSynthesis incorporates "sub-strategies" that are composed to form CSDs now
2. GeneratedCSD.dfy is added as a "template" CSD file that Qwen would fill in later

next steps include:
1. adding code for qwen to fill in GeneratedCSD.dfy
2. automating the compilation of that to python, running in python and the overall feedback loop
3. testing that feedback loop against gsm symbolic

proofs/VerifiedAgentSynthesis-py-py/VerifiedDecoderAgent.py
@@ -1,0 +1,570 @@
+import sys
+from typing import Callable, Any, TypeVar, NamedTuple
+from math import floor
+from itertools import count
+
+import module_ as module_
+import _dafny as _dafny
+import System_ as System_
+
+# Module: VerifiedDecoderAgent
+
+class default__:
+    def  __init__(self):
+        pass
+
+    @staticmethod
+    def CRANEStyle(startDelim, endDelim):
+        return Strategy_Window(startDelim, endDelim, TokenConstraint_GrammarMask(), TokenConstraint_NoConstraint())
+
+    @staticmethod
+    def RetryThenConstrained(k):
+        return Strategy_TryK(k, Attempt_Unconstrained(), CheckPredicate_ParseOk(), Strategy_Constrained(TokenConstraint_GrammarMask()))
+
+    @staticmethod
+    def BestOfNWithRepair(n, repairRules):
+        return Strategy_BestOfN(n, Strategy_TryK(1, Attempt_WithRepair(Attempt_Unconstrained(), repairRules), CheckPredicate_ParseOk(), Strategy_Constrained(TokenConstraint_GrammarMask())), CheckPredicate_ParseOk())
+
+    @staticmethod
+    def GuaranteesValidOutput(strategy):
+        source0_ = strategy
+        if True:
+            if source0_.is_Constrained:
+                return True
+        if True:
+            if source0_.is_Window:
+                return True
+        if True:
+            if source0_.is_TryK:
+                d_0_fallback_ = source0_.fallback
+                return default__.GuaranteesValidOutput(d_0_fallback_)
+        if True:
+            if source0_.is_Cascade:
+                d_1_strategies_ = source0_.strategies
+                return ((len(d_1_strategies_)) > (0)) and (default__.GuaranteesValidOutput((d_1_strategies_)[(len(d_1_strategies_)) - (1)]))
+        if True:
+            if source0_.is_BestOfN:
+                d_2_base_ = source0_.base
+                return default__.GuaranteesValidOutput(d_2_base_)
+        if True:
+            return False
+
+
+class LM:
+    def  __init__(self):
+        self.Logits: _dafny.Seq = _dafny.Seq({})
+        self._Tokens: _dafny.Seq = _dafny.Seq({})
+        self._Ids: _dafny.Seq = _dafny.Seq({})
+        pass
+
+    def __dafnystr__(self) -> str:
+        return "VerifiedDecoderAgent.LM"
+    def ValidTokensIdsLogits(self):
+        def lambda0_(forall_var_0_):
+            def lambda1_(forall_var_1_):
+                d_1_j_: int = forall_var_1_
+                return not (((((0) <= (d_0_i_)) and ((d_0_i_) < (len((self).Tokens)))) and (((0) <= (d_1_j_)) and ((d_1_j_) < (len((self).Tokens))))) and ((d_0_i_) != (d_1_j_))) or ((((self).Tokens)[d_0_i_]) != (((self).Tokens)[d_1_j_]))
+
+            d_0_i_: int = forall_var_0_
+            return _dafny.quantifier(_dafny.IntegerRange(0, len((self).Tokens)), True, lambda1_)
+
+        def lambda2_(forall_var_2_):
+            def lambda3_(exists_var_0_):
+                d_3_i_: int = exists_var_0_
+                return (((0) <= (d_3_i_)) and ((d_3_i_) < (len((self).Ids)))) and ((((self).Tokens)[d_3_i_]) == (d_2_token_))
+
+            d_2_token_: _dafny.Seq = forall_var_2_
+            return not ((d_2_token_) in ((self).Tokens)) or (_dafny.quantifier(_dafny.IntegerRange(0, len((self).Ids)), False, lambda3_))
+
+        def lambda4_(forall_var_3_):
+            d_4_i_: int = forall_var_3_
+            return not (((0) <= (d_4_i_)) and ((d_4_i_) < (len((self).Ids)))) or (((d_4_i_) == (((self).Ids)[d_4_i_])) and ((d_4_i_) in ((self).Ids)))
+
+        def lambda5_(forall_var_4_):
+            d_5_i_: int = forall_var_4_
+            return not (((0) <= (d_5_i_)) and ((d_5_i_) < (len(self.Logits)))) or ((((self.Logits)[d_5_i_]) <= (_dafny.BigRational('1e9'))) and (((self.Logits)[d_5_i_]) >= (_dafny.BigRational('-1e9'))))
+
+        return (((((((len((self).Tokens)) == (len((self).Ids))) and ((len((self).Ids)) == (len(self.Logits)))) and (((len((self).Ids)) > (0)) and ((((self).Ids)[0]) == (0)))) and (_dafny.quantifier(_dafny.IntegerRange(0, len((self).Tokens)), True, lambda0_))) and (_dafny.quantifier(((self).Tokens).UniqueElements, True, lambda2_))) and (_dafny.quantifier(_dafny.IntegerRange(0, len((self).Ids)), True, lambda4_))) and (_dafny.quantifier(_dafny.IntegerRange(0, len(self.Logits)), True, lambda5_))
+
+    def IdToToken(self, id_):
+        return ((self).Tokens)[id_]
+
+    def TokenToId(self, token):
+        return (self).TokenToIdRecursive(token, (self).Tokens)
+
+    def TokenToIdRecursive(self, token, tokens):
+        d_0___accumulator_ = 0
+        _this = self
+        while True:
+            with _dafny.label():
+                if ((tokens)[0]) == (token):
+                    return (0) + (d_0___accumulator_)
+                elif True:
+                    d_0___accumulator_ = (d_0___accumulator_) + (1)
+                    in0_ = _this
+                    in1_ = token
+                    in2_ = _dafny.SeqWithoutIsStrInference((tokens)[1::])
+                    _this = in0_
+                    
+                    token = in1_
+                    tokens = in2_
+                    raise _dafny.TailCall()
+                break
+
+    def IdToLogit(self, id_):
+        return (self.Logits)[id_]
+
+    def TokenToLogit(self, token):
+        return (self).IdToLogit((self).TokenToId(token))
+
+    def TokensToLogits(self, tokens):
+        d_0___accumulator_ = _dafny.SeqWithoutIsStrInference([])
+        _this = self
+        while True:
+            with _dafny.label():
+                if (len(tokens)) == (1):
+                    return (d_0___accumulator_) + (_dafny.SeqWithoutIsStrInference([(_this).TokenToLogit((tokens)[0])]))
+                elif True:
+                    d_0___accumulator_ = (d_0___accumulator_) + (_dafny.SeqWithoutIsStrInference([(_this).TokenToLogit((tokens)[0])]))
+                    in0_ = _this
+                    in1_ = _dafny.SeqWithoutIsStrInference((tokens)[1::])
+                    _this = in0_
+                    
+                    tokens = in1_
+                    raise _dafny.TailCall()
+                break
+
+    def IdsToLogits(self, ids):
+        d_0___accumulator_ = _dafny.SeqWithoutIsStrInference([])
+        _this = self
+        while True:
+            with _dafny.label():
+                if (len(ids)) == (1):
+                    return (d_0___accumulator_) + (_dafny.SeqWithoutIsStrInference([(_this).IdToLogit((ids)[0])]))
+                elif True:
+                    d_0___accumulator_ = (d_0___accumulator_) + (_dafny.SeqWithoutIsStrInference([(_this).IdToLogit((ids)[0])]))
+                    in0_ = _this
+                    in1_ = _dafny.SeqWithoutIsStrInference((ids)[1::])
+                    _this = in0_
+                    
+                    ids = in1_
+                    raise _dafny.TailCall()
+                break
+
+    def MaskToken(self, token):
+        d_0_id_: int
+        d_0_id_ = (self).TokenToId(token)
+        (self).Logits = ((_dafny.SeqWithoutIsStrInference((self.Logits)[:d_0_id_:])) + (_dafny.SeqWithoutIsStrInference([_dafny.BigRational('0e0')]))) + (_dafny.SeqWithoutIsStrInference((self.Logits)[(d_0_id_) + (1)::]))
+
+    def MaskTokens(self, tokens):
+        d_0_N_: int
+        d_0_N_ = len(tokens)
+        d_1_i_: int
+        d_1_i_ = 0
+        while (d_1_i_) < (d_0_N_):
+            (self).MaskToken((tokens)[d_1_i_])
+            d_1_i_ = (d_1_i_) + (1)
+
+    @property
+    def Tokens(self):
+        return self._Tokens
+    @property
+    def Ids(self):
+        return self._Ids
+
+class Parser:
+    def  __init__(self):
+        pass
+
+    def __dafnystr__(self) -> str:
+        return "VerifiedDecoderAgent.Parser"
+
+class TokenConstraint:
+    @classmethod
+    def default(cls, ):
+        return lambda: TokenConstraint_GrammarMask()
+    def __ne__(self, __o: object) -> bool:
+        return not self.__eq__(__o)
+    @property
+    def is_GrammarMask(self) -> bool:
+        return isinstance(self, TokenConstraint_GrammarMask)
+    @property
+    def is_Lookahead(self) -> bool:
+        return isinstance(self, TokenConstraint_Lookahead)
+    @property
+    def is_LengthBound(self) -> bool:
+        return isinstance(self, TokenConstraint_LengthBound)
+    @property
+    def is_BanTokens(self) -> bool:
+        return isinstance(self, TokenConstraint_BanTokens)
+    @property
+    def is_AllowOnlyTokens(self) -> bool:
+        return isinstance(self, TokenConstraint_AllowOnlyTokens)
+    @property
+    def is_Intersect(self) -> bool:
+        return isinstance(self, TokenConstraint_Intersect)
+    @property
+    def is_Union(self) -> bool:
+        return isinstance(self, TokenConstraint_Union)
+    @property
+    def is_NoConstraint(self) -> bool:
+        return isinstance(self, TokenConstraint_NoConstraint)
+
+class TokenConstraint_GrammarMask(TokenConstraint, NamedTuple('GrammarMask', [])):
+    def __dafnystr__(self) -> str:
+        return f'VerifiedDecoderAgent.TokenConstraint.GrammarMask'
+    def __eq__(self, __o: object) -> bool:
+        return isinstance(__o, TokenConstraint_GrammarMask)
+    def __hash__(self) -> int:
+        return super().__hash__()
+
+class TokenConstraint_Lookahead(TokenConstraint, NamedTuple('Lookahead', [('depth', Any)])):
+    def __dafnystr__(self) -> str:
+        return f'VerifiedDecoderAgent.TokenConstraint.Lookahead({_dafny.string_of(self.depth)})'
+    def __eq__(self, __o: object) -> bool:
+        return isinstance(__o, TokenConstraint_Lookahead) and self.depth == __o.depth
+    def __hash__(self) -> int:
+        return super().__hash__()
+
+class TokenConstraint_LengthBound(TokenConstraint, NamedTuple('LengthBound', [('min_', Any), ('max_', Any)])):
+    def __dafnystr__(self) -> str:
+        return f'VerifiedDecoderAgent.TokenConstraint.LengthBound({_dafny.string_of(self.min_)}, {_dafny.string_of(self.max_)})'
+    def __eq__(self, __o: object) -> bool:
+        return isinstance(__o, TokenConstraint_LengthBound) and self.min_ == __o.min_ and self.max_ == __o.max_
+    def __hash__(self) -> int:
+        return super().__hash__()
+
+class TokenConstraint_BanTokens(TokenConstraint, NamedTuple('BanTokens', [('banned', Any)])):
+    def __dafnystr__(self) -> str:
+        return f'VerifiedDecoderAgent.TokenConstraint.BanTokens({_dafny.string_of(self.banned)})'
+    def __eq__(self, __o: object) -> bool:
+        return isinstance(__o, TokenConstraint_BanTokens) and self.banned == __o.banned
+    def __hash__(self) -> int:
+        return super().__hash__()
+
+class TokenConstraint_AllowOnlyTokens(TokenConstraint, NamedTuple('AllowOnlyTokens', [('allowed', Any)])):
+    def __dafnystr__(self) -> str:
+        return f'VerifiedDecoderAgent.TokenConstraint.AllowOnlyTokens({_dafny.string_of(self.allowed)})'
+    def __eq__(self, __o: object) -> bool:
+        return isinstance(__o, TokenConstraint_AllowOnlyTokens) and self.allowed == __o.allowed
+    def __hash__(self) -> int:
+        return super().__hash__()
+
+class TokenConstraint_Intersect(TokenConstraint, NamedTuple('Intersect', [('a', Any), ('b', Any)])):
+    def __dafnystr__(self) -> str:
+        return f'VerifiedDecoderAgent.TokenConstraint.Intersect({_dafny.string_of(self.a)}, {_dafny.string_of(self.b)})'
+    def __eq__(self, __o: object) -> bool:
+        return isinstance(__o, TokenConstraint_Intersect) and self.a == __o.a and self.b == __o.b
+    def __hash__(self) -> int:
+        return super().__hash__()
+
+class TokenConstraint_Union(TokenConstraint, NamedTuple('Union', [('a', Any), ('b', Any)])):
+    def __dafnystr__(self) -> str:
+        return f'VerifiedDecoderAgent.TokenConstraint.Union({_dafny.string_of(self.a)}, {_dafny.string_of(self.b)})'
+    def __eq__(self, __o: object) -> bool:
+        return isinstance(__o, TokenConstraint_Union) and self.a == __o.a and self.b == __o.b
+    def __hash__(self) -> int:
+        return super().__hash__()
+
+class TokenConstraint_NoConstraint(TokenConstraint, NamedTuple('NoConstraint', [])):
+    def __dafnystr__(self) -> str:
+        return f'VerifiedDecoderAgent.TokenConstraint.NoConstraint'
+    def __eq__(self, __o: object) -> bool:
+        return isinstance(__o, TokenConstraint_NoConstraint)
+    def __hash__(self) -> int:
+        return super().__hash__()
+
+
+class RepairRules:
+    @classmethod
+    def default(cls, ):
+        return lambda: RepairRules_BracketBalance()
+    def __ne__(self, __o: object) -> bool:
+        return not self.__eq__(__o)
+    @property
+    def is_BracketBalance(self) -> bool:
+        return isinstance(self, RepairRules_BracketBalance)
+    @property
+    def is_QuoteFix(self) -> bool:
+        return isinstance(self, RepairRules_QuoteFix)
+    @property
+    def is_WhitespaceNormalize(self) -> bool:
+        return isinstance(self, RepairRules_WhitespaceNormalize)
+    @property
+    def is_ComposedRepair(self) -> bool:
+        return isinstance(self, RepairRules_ComposedRepair)
+    @property
+    def is_NoRepair(self) -> bool:
+        return isinstance(self, RepairRules_NoRepair)
+
+class RepairRules_BracketBalance(RepairRules, NamedTuple('BracketBalance', [])):
+    def __dafnystr__(self) -> str:
+        return f'VerifiedDecoderAgent.RepairRules.BracketBalance'
+    def __eq__(self, __o: object) -> bool:
+        return isinstance(__o, RepairRules_BracketBalance)
+    def __hash__(self) -> int:
+        return super().__hash__()
+
+class RepairRules_QuoteFix(RepairRules, NamedTuple('QuoteFix', [])):
+    def __dafnystr__(self) -> str:
+        return f'VerifiedDecoderAgent.RepairRules.QuoteFix'
+    def __eq__(self, __o: object) -> bool:
+        return isinstance(__o, RepairRules_QuoteFix)
+    def __hash__(self) -> int:
+        return super().__hash__()
+
+class RepairRules_WhitespaceNormalize(RepairRules, NamedTuple('WhitespaceNormalize', [])):
+    def __dafnystr__(self) -> str:
+        return f'VerifiedDecoderAgent.RepairRules.WhitespaceNormalize'
+    def __eq__(self, __o: object) -> bool:
+        return isinstance(__o, RepairRules_WhitespaceNormalize)
+    def __hash__(self) -> int:
+        return super().__hash__()
+
+class RepairRules_ComposedRepair(RepairRules, NamedTuple('ComposedRepair', [('a', Any), ('b', Any)])):
+    def __dafnystr__(self) -> str:
+        return f'VerifiedDecoderAgent.RepairRules.ComposedRepair({_dafny.string_of(self.a)}, {_dafny.string_of(self.b)})'
+    def __eq__(self, __o: object) -> bool:
+        return isinstance(__o, RepairRules_ComposedRepair) and self.a == __o.a and self.b == __o.b
+    def __hash__(self) -> int:
+        return super().__hash__()
+
+class RepairRules_NoRepair(RepairRules, NamedTuple('NoRepair', [])):
+    def __dafnystr__(self) -> str:
+        return f'VerifiedDecoderAgent.RepairRules.NoRepair'
+    def __eq__(self, __o: object) -> bool:
+        return isinstance(__o, RepairRules_NoRepair)
+    def __hash__(self) -> int:
+        return super().__hash__()
+
+
+
+class SeqOperation:
+    @classmethod
+    def default(cls, ):
+        return lambda: SeqOperation_Repair(RepairRules.default()())
+    def __ne__(self, __o: object) -> bool:
+        return not self.__eq__(__o)
+    @property
+    def is_Repair(self) -> bool:
+        return isinstance(self, SeqOperation_Repair)
+    @property
+    def is_PrefixCompleteOp(self) -> bool:
+        return isinstance(self, SeqOperation_PrefixCompleteOp)
+    @property
+    def is_ValidateOp(self) -> bool:
+        return isinstance(self, SeqOperation_ValidateOp)
+    @property
+    def is_Identity(self) -> bool:
+        return isinstance(self, SeqOperation_Identity)
+
+class SeqOperation_Repair(SeqOperation, NamedTuple('Repair', [('rules', Any)])):
+    def __dafnystr__(self) -> str:
+        return f'VerifiedDecoderAgent.SeqOperation.Repair({_dafny.string_of(self.rules)})'
+    def __eq__(self, __o: object) -> bool:
+        return isinstance(__o, SeqOperation_Repair) and self.rules == __o.rules
+    def __hash__(self) -> int:
+        return super().__hash__()
+
+class SeqOperation_PrefixCompleteOp(SeqOperation, NamedTuple('PrefixCompleteOp', [('constraint', Any)])):
+    def __dafnystr__(self) -> str:
+        return f'VerifiedDecoderAgent.SeqOperation.PrefixCompleteOp({_dafny.string_of(self.constraint)})'
+    def __eq__(self, __o: object) -> bool:
+        return isinstance(__o, SeqOperation_PrefixCompleteOp) and self.constraint == __o.constraint
+    def __hash__(self) -> int:
+        return super().__hash__()
+
+class SeqOperation_ValidateOp(SeqOperation, NamedTuple('ValidateOp', [('pred', Any)])):
+    def __dafnystr__(self) -> str:
+        return f'VerifiedDecoderAgent.SeqOperation.ValidateOp({_dafny.string_of(self.pred)})'
+    def __eq__(self, __o: object) -> bool:
+        return isinstance(__o, SeqOperation_ValidateOp) and self.pred == __o.pred
+    def __hash__(self) -> int:
+        return super().__hash__()
+
+class SeqOperation_Identity(SeqOperation, NamedTuple('Identity', [])):
+    def __dafnystr__(self) -> str:
+        return f'VerifiedDecoderAgent.SeqOperation.Identity'
+    def __eq__(self, __o: object) -> bool:
+        return isinstance(__o, SeqOperation_Identity)
+    def __hash__(self) -> int:
+        return super().__hash__()
+
+
+class CheckPredicate:
+    @classmethod
+    def default(cls, ):
+        return lambda: CheckPredicate_ParseOk()
+    def __ne__(self, __o: object) -> bool:
+        return not self.__eq__(__o)
+    @property
+    def is_ParseOk(self) -> bool:
+        return isinstance(self, CheckPredicate_ParseOk)
+    @property
+    def is_SemanticOk(self) -> bool:
+        return isinstance(self, CheckPredicate_SemanticOk)
+    @property
+    def is_Both(self) -> bool:
+        return isinstance(self, CheckPredicate_Both)
+    @property
+    def is_Either(self) -> bool:
+        return isinstance(self, CheckPredicate_Either)
+
+class CheckPredicate_ParseOk(CheckPredicate, NamedTuple('ParseOk', [])):
+    def __dafnystr__(self) -> str:
+        return f'VerifiedDecoderAgent.CheckPredicate.ParseOk'
+    def __eq__(self, __o: object) -> bool:
+        return isinstance(__o, CheckPredicate_ParseOk)
+    def __hash__(self) -> int:
+        return super().__hash__()
+
+class CheckPredicate_SemanticOk(CheckPredicate, NamedTuple('SemanticOk', [('pred', Any)])):
+    def __dafnystr__(self) -> str:
+        return f'VerifiedDecoderAgent.CheckPredicate.SemanticOk({_dafny.string_of(self.pred)})'
+    def __eq__(self, __o: object) -> bool:
+        return isinstance(__o, CheckPredicate_SemanticOk) and self.pred == __o.pred
+    def __hash__(self) -> int:
+        return super().__hash__()
+
+class CheckPredicate_Both(CheckPredicate, NamedTuple('Both', [('a', Any), ('b', Any)])):
+    def __dafnystr__(self) -> str:
+        return f'VerifiedDecoderAgent.CheckPredicate.Both({_dafny.string_of(self.a)}, {_dafny.string_of(self.b)})'
+    def __eq__(self, __o: object) -> bool:
+        return isinstance(__o, CheckPredicate_Both) and self.a == __o.a and self.b == __o.b
+    def __hash__(self) -> int:
+        return super().__hash__()
+
+class CheckPredicate_Either(CheckPredicate, NamedTuple('Either', [('a', Any), ('b', Any)])):
+    def __dafnystr__(self) -> str:
+        return f'VerifiedDecoderAgent.CheckPredicate.Either({_dafny.string_of(self.a)}, {_dafny.string_of(self.b)})'
+    def __eq__(self, __o: object) -> bool:
+        return isinstance(__o, CheckPredicate_Either) and self.a == __o.a and self.b == __o.b
+    def __hash__(self) -> int:
+        return super().__hash__()
+
+
+class Attempt:
+    @classmethod
+    def default(cls, ):
+        return lambda: Attempt_Unconstrained()
+    def __ne__(self, __o: object) -> bool:
+        return not self.__eq__(__o)
+    @property
+    def is_Unconstrained(self) -> bool:
+        return isinstance(self, Attempt_Unconstrained)
+    @property
+    def is_ConstrainedAttempt(self) -> bool:
+        return isinstance(self, Attempt_ConstrainedAttempt)
+    @property
+    def is_WithRepair(self) -> bool:
+        return isinstance(self, Attempt_WithRepair)
+    @property
+    def is_WithSeqOp(self) -> bool:
+        return isinstance(self, Attempt_WithSeqOp)
+
+class Attempt_Unconstrained(Attempt, NamedTuple('Unconstrained', [])):
+    def __dafnystr__(self) -> str:
+        return f'VerifiedDecoderAgent.Attempt.Unconstrained'
+    def __eq__(self, __o: object) -> bool:
+        return isinstance(__o, Attempt_Unconstrained)
+    def __hash__(self) -> int:
+        return super().__hash__()
+
+class Attempt_ConstrainedAttempt(Attempt, NamedTuple('ConstrainedAttempt', [('constraint', Any)])):
+    def __dafnystr__(self) -> str:
+        return f'VerifiedDecoderAgent.Attempt.ConstrainedAttempt({_dafny.string_of(self.constraint)})'
+    def __eq__(self, __o: object) -> bool:
+        return isinstance(__o, Attempt_ConstrainedAttempt) and self.constraint == __o.constraint
+    def __hash__(self) -> int:
+        return super().__hash__()
+
+class Attempt_WithRepair(Attempt, NamedTuple('WithRepair', [('base', Any), ('rules', Any)])):
+    def __dafnystr__(self) -> str:
+        return f'VerifiedDecoderAgent.Attempt.WithRepair({_dafny.string_of(self.base)}, {_dafny.string_of(self.rules)})'
+    def __eq__(self, __o: object) -> bool:
+        return isinstance(__o, Attempt_WithRepair) and self.base == __o.base and self.rules == __o.rules
+    def __hash__(self) -> int:
+        return super().__hash__()
+
+class Attempt_WithSeqOp(Attempt, NamedTuple('WithSeqOp', [('base', Any), ('op', Any)])):
+    def __dafnystr__(self) -> str:
+        return f'VerifiedDecoderAgent.Attempt.WithSeqOp({_dafny.string_of(self.base)}, {_dafny.string_of(self.op)})'
+    def __eq__(self, __o: object) -> bool:
+        return isinstance(__o, Attempt_WithSeqOp) and self.base == __o.base and self.op == __o.op
+    def __hash__(self) -> int:
+        return super().__hash__()
+
+
+class Strategy:
+    @classmethod
+    def default(cls, ):
+        return lambda: Strategy_Window(_dafny.SeqWithoutIsStrInference(map(_dafny.CodePoint, "")), _dafny.SeqWithoutIsStrInference(map(_dafny.CodePoint, "")), TokenConstraint.default()(), TokenConstraint.default()())
+    def __ne__(self, __o: object) -> bool:
+        return not self.__eq__(__o)
+    @property
+    def is_Window(self) -> bool:
+        return isinstance(self, Strategy_Window)
+    @property
+    def is_TryK(self) -> bool:
+        return isinstance(self, Strategy_TryK)
+    @property
+    def is_Cascade(self) -> bool:
+        return isinstance(self, Strategy_Cascade)
+    @property
+    def is_BestOfN(self) -> bool:
+        return isinstance(self, Strategy_BestOfN)
+    @property
+    def is_Constrained(self) -> bool:
+        return isinstance(self, Strategy_Constrained)
+    @property
+    def is_Free(self) -> bool:
+        return isinstance(self, Strategy_Free)
+
+class Strategy_Window(Strategy, NamedTuple('Window', [('startDelim', Any), ('endDelim', Any), ('inside', Any), ('outside', Any)])):
+    def __dafnystr__(self) -> str:
+        return f'VerifiedDecoderAgent.Strategy.Window({self.startDelim.VerbatimString(True)}, {self.endDelim.VerbatimString(True)}, {_dafny.string_of(self.inside)}, {_dafny.string_of(self.outside)})'
+    def __eq__(self, __o: object) -> bool:
+        return isinstance(__o, Strategy_Window) and self.startDelim == __o.startDelim and self.endDelim == __o.endDelim and self.inside == __o.inside and self.outside == __o.outside
+    def __hash__(self) -> int:
+        return super().__hash__()
+
+class Strategy_TryK(Strategy, NamedTuple('TryK', [('k', Any), ('attempt', Any), ('check', Any), ('fallback', Any)])):
+    def __dafnystr__(self) -> str:
+        return f'VerifiedDecoderAgent.Strategy.TryK({_dafny.string_of(self.k)}, {_dafny.string_of(self.attempt)}, {_dafny.string_of(self.check)}, {_dafny.string_of(self.fallback)})'
+    def __eq__(self, __o: object) -> bool:
+        return isinstance(__o, Strategy_TryK) and self.k == __o.k and self.attempt == __o.attempt and self.check == __o.check and self.fallback == __o.fallback
+    def __hash__(self) -> int:
+        return super().__hash__()
+
+class Strategy_Cascade(Strategy, NamedTuple('Cascade', [('strategies', Any), ('check', Any)])):
+    def __dafnystr__(self) -> str:
+        return f'VerifiedDecoderAgent.Strategy.Cascade({_dafny.string_of(self.strategies)}, {_dafny.string_of(self.check)})'
+    def __eq__(self, __o: object) -> bool:
+        return isinstance(__o, Strategy_Cascade) and self.strategies == __o.strategies and self.check == __o.check
+    def __hash__(self) -> int:
+        return super().__hash__()
+
+class Strategy_BestOfN(Strategy, NamedTuple('BestOfN', [('n', Any), ('base', Any), ('check', Any)])):
+    def __dafnystr__(self) -> str:
+        return f'VerifiedDecoderAgent.Strategy.BestOfN({_dafny.string_of(self.n)}, {_dafny.string_of(self.base)}, {_dafny.string_of(self.check)})'
+    def __eq__(self, __o: object) -> bool:
+        return isinstance(__o, Strategy_BestOfN) and self.n == __o.n and self.base == __o.base and self.check == __o.check
+    def __hash__(self) -> int:
+        return super().__hash__()
+
+class Strategy_Constrained(Strategy, NamedTuple('Constrained', [('constraint', Any)])):
+    def __dafnystr__(self) -> str:
+        return f'VerifiedDecoderAgent.Strategy.Constrained({_dafny.string_of(self.constraint)})'
+    def __eq__(self, __o: object) -> bool:
+        return isinstance(__o, Strategy_Constrained) and self.constraint == __o.constraint
+    def __hash__(self) -> int:
+        return super().__hash__()
+
+class Strategy_Free(Strategy, NamedTuple('Free', [])):
+    def __dafnystr__(self) -> str:
+        return f'VerifiedDecoderAgent.Strategy.Free'
+    def __eq__(self, __o: object) -> bool:
+        return isinstance(__o, Strategy_Free)
+    def __hash__(self) -> int:
+        return super().__hash__()
+
